src/frontends/lean/tactic_notation.h
@@ -13,6 +13,7 @@ expr parse_curly_begin_end_expr(parser & p, pos_info const & pos);
 expr parse_begin_end(parser & p, unsigned, expr const *, pos_info const & pos);
 expr parse_by(parser & p, unsigned, expr const *, pos_info const & pos);
 expr parse_interactive_tactic_block(parser & p, unsigned, expr const *, pos_info const & pos);
+expr parse_nested_interactive_tactic(parser & p, name const & tac_class, bool use_istep);
 void initialize_tactic_notation();
 void finalize_tactic_notation();
 }
