src/library/constants.h
@@ -180,6 +180,7 @@ name const & get_is_commutative_comm_name();
 name const & get_ite_name();
 name const & get_lean_parser_name();
 name const & get_lean_parser_pexpr_name();
+name const & get_lean_parser_reflectable_expr_name();
 name const & get_lean_parser_tk_name();
 name const & get_left_distrib_name();
 name const & get_left_comm_name();
