tests/lean/run/parser_itactic.lean
@@ -1,0 +1,30 @@
+open tactic
+
+namespace tactic.interactive
+
+meta def my_tac (p : interactive.parse lean.parser.itactic) : tactic unit :=
+p
+
+meta def my_tac_optional (p : interactive.parse (optional lean.parser.itactic)) : tactic unit :=
+match p with
+| some p := p
+| none := tactic.trace "nothing"
+end
+
+end tactic.interactive
+
+meta def quote_tac : tactic unit := `[my_tac {tactic.trace "hi2"}]
+meta def quote_tac_optional : tactic unit := `[my_tac_optional]
+
+example : true := begin
+    my_tac {tactic.trace "hi"},
+
+    my_tac_optional {tactic.trace "hi"},
+    my_tac_optional {},
+    my_tac_optional,
+
+    quote_tac,
+    quote_tac_optional,
+
+    trivial
+end
